aneris/examples/snapshot_isolation/proof/instantiation/instantiation_of_resources.v
@@ -1,0 +1,89 @@
+From iris.algebra Require Import agree auth excl gmap updates local_updates.
+From iris.algebra.lib Require Import mono_list.
+From iris.base_logic.lib Require Import mono_nat ghost_map.
+From iris.base_logic Require Import invariants.
+From iris.bi.lib Require Import fractional.
+From iris.proofmode Require Import tactics.
+From aneris.prelude Require Import list.
+From aneris.algebra Require Import monotone.
+From aneris.aneris_lang Require Import lang resources resources inject.
+From aneris.lib Require Import gen_heap_light.
+From aneris.aneris_lang.lib Require Import
+     list_proof monitor_proof lock_proof map_proof.
+From aneris.aneris_lang.lib.serialization Require Import serialization_proof.
+From aneris.examples.reliable_communication.lib.mt_server Require Import user_params.
+From aneris.examples.snapshot_isolation.specs Require Import user_params resources.
+From aneris.examples.snapshot_isolation.proof
+     Require Import time events model.
+From aneris.examples.snapshot_isolation.proof.resources
+     Require Import resource_algebras server_resources proxy_resources
+     global_invariant.
+
+
+Section Session_Resources_intantiation.
+  Context `{!anerisG Mdl Σ, !IDBG Σ, !MTS_resources}.
+  Context `{!User_params}.
+  Context (clients : gset socket_address).
+  Context (γKnownClients γGauth γGsnap γT : gname).
+  Context (srv_si : message → iProp Σ) (SrvInit : iProp Σ).
+
+  Definition to_hist (h : list write_event) : list val := (λ e, e.(we_val)) <$> h.
+
+  Definition to_local_state (s : proxy_state) : local_state :=
+    match s with
+      PSCanStart => CanStart
+    | PSActive m => Active ((λ h, to_hist h) <$> m)
+    end.
+
+  Lemma to_hist_prefix_mono hw hw' :
+    hw `suffix_of` hw' →  to_hist hw `suffix_of` to_hist hw'.
+  Proof.
+  Admitted.
+
+  Definition GlobalInv_def : iProp Σ :=
+    Global_Inv clients γKnownClients γGauth γGsnap γT.
+
+  Definition OwnMemKey_def k h : iProp Σ :=
+    ∃ hw, ownMemUser γGauth γGsnap k hw ∗ ⌜h = to_hist hw⌝.
+
+  Definition ConnectionState_def c s : iProp Σ :=
+    ∃ sp, connection_state  γGsnap γT γKnownClients c sp ∗ ⌜s = to_local_state sp⌝.
+
+  Definition Seen_def k h : iProp Σ :=
+    ∃ hw, ownMemSeen γGsnap k hw ∗ ⌜h = to_hist hw⌝.
+
+
+  Global Program Instance session_resources_instance : SI_resources Mdl Σ :=
+    {|
+      GlobalInv :=  GlobalInv_def;
+      OwnMemKey k h := OwnMemKey_def k h;
+      OwnLocalKey k c vo := ownCacheUser γKnownClients k c vo;
+      ConnectionState c s := ConnectionState_def c s;
+      IsConnected c := is_connected γGsnap γT γKnownClients c;
+      KeyUpdStatus c k b :=  key_upd_status γKnownClients c k b;
+      Seen k h := Seen_def k h;
+      KVS_si := srv_si;
+      KVS_Init := SrvInit;
+      KVS_ClientCanConnect sa := client_can_connect γKnownClients sa;
+      OwnLocalKey_serializable k c v :=
+      own_cache_user_serializable γGsnap γT γKnownClients k c v;
+      (* Seen_valid E k h h' :=  *) |}.
+  Next Obligation.
+    iIntros (E k h h' Hcl) "#Hinv (#Hs & Hk)".
+    iDestruct "Hs" as (hw) "(Hs & %Heq1)".
+    iDestruct "Hk" as (hw') "(Hk & %Heq2)".
+    unfold OwnMemKey_def, GlobalInv_def.
+    iDestruct
+      (ownMemSeen_valid clients γKnownClients γGauth γGsnap γT E k hw hw' with
+        "[$] [$]")
+      as "Hp"; try eauto.
+    iMod ("Hp" with "[$Hk]") as "(Hp & %Hpre)".
+    iModIntro.
+    iSplit; first eauto.
+    iPureIntro.
+    simplify_eq /=.
+    (** FixMe in either in the resources or in resources definition. *)
+    admit.
+    Admitted.
+
+End Session_Resources_intantiation.
