aneris/examples/snapshot_isolation/proof/resources/global_invariant.v
@@ -11,25 +11,31 @@ From aneris.lib Require Import gen_heap_light.
 From aneris.aneris_lang.lib Require Import
      list_proof monitor_proof lock_proof map_proof.
 From aneris.aneris_lang.lib.serialization Require Import serialization_proof.
+From aneris.examples.reliable_communication.lib.mt_server Require Import user_params.
 From aneris.examples.snapshot_isolation.specs Require Import user_params.
 From aneris.examples.snapshot_isolation.proof
      Require Import time events model.
 From aneris.examples.snapshot_isolation.proof.resources
-     Require Import resource_algebras server_resources.
+     Require Import resource_algebras server_resources proxy_resources.
 
 
 Section Global_Invariant.
 
-  Context `{!anerisG Mdl Σ, !User_params, !IDBG Σ}.
+  Context `{!anerisG Mdl Σ, !User_params, !IDBG Σ, !MTS_resources}.
+  Context (clients : gset socket_address).
+  Context (γKnownClients : gname).
   Context (γGauth γGsnap γT : gname).
 
   (* ------------------------------------------------------------------------ *)
   (** Definition of the global invariant. *)
   Definition global_inv_def : iProp Σ :=
     ∃ (M : gmap Key (list write_event))
-      (T : Time),
+      (T : Time)
+      (gM : gmap socket_address gname),
       ownMemGlobal γGauth γGsnap M ∗
       ownTimeGlobal γT T ∗
+      connected_clients γKnownClients gM ∗
+      ⌜dom gM = clients⌝ ∗
       ⌜kvs_valid M T⌝.
 
   Definition Global_Inv : iProp Σ :=
@@ -42,46 +48,61 @@ Section Global_Invariant.
     nclose KVS_InvName ⊆ E →
     Global_Inv ⊢
     ownMemSeen γGsnap k h -∗ ownMemUser γGauth γGsnap k h' ={E}=∗
-    ownMemUser γGauth γGsnap  k h' ∗ ⌜h `prefix_of` h'⌝.
+    ownMemUser γGauth γGsnap k h' ∗ ⌜h `prefix_of` h'⌝.
   Proof.
     iIntros (?) "#Hginv #Hm Hu".
     iDestruct "Hu" as "(Hu & #Hum)".
     rewrite /Global_Inv /ownMemSeen.
-    iInv KVS_InvName as (M T) ">((HmemA & HmemM) & ? & %Hvalid)" "Hcl".
+    iInv KVS_InvName as (M T gM) ">((HmemA & HmemM) & ? & ? & ? & %Hvalid)" "Hcl".
     iDestruct (ownMemSeen_lookup with "HmemM Hm") as (h1) "(%Hh1 & %Hh2)".
     iDestruct (ghost_map_lookup with "HmemA Hu") as "%Hh3".
     simplify_eq /=.
     iFrame "#". iFrame.
     iMod ("Hcl" with "[-]") as "_".
-    { iNext. do 2 iExists _. by iFrame. }
+    { iNext. do 3 iExists _. by iFrame. }
     by iModIntro.
   Qed.
 
-  (** FIXME: Maybe don't need the GlobalInv,
-      in which case update the specs.resources *)
-  (* Lemma ConnectionState_relation E k r ms h :
-      ↑KVS_InvName ⊆ E ->
-      GlobalInv ⊢
-      ConnectionState r (Active ms) -∗ k ↦ₖ h ={E}=∗
-      ConnectionState r (Active ms) ∗ k ↦ₖ h ∗
-      ⌜k ∈ dom ms →
-      ∀ h', ms !! k = Some h' → h' ≤ₛ h ⌝; *)
 
-  (** FIXME: Maybe don't need the GlobalInv,
-      in which case update the specs.resources *)
-  (* OwnMemKey_OwnLocalKey_coh k h vo c E :
-        ↑KVS_InvName ⊆ E ->
-        h ≠ [] ->
-        GlobalInv ⊢
-        k ↦ₖ h -∗ k ↦{c} vo ={E}=∗ k ↦ₖ h -∗ k ↦{c} vo ∗ ⌜is_Some vo⌝;  *)
+  (* (** NB: not sure we will use this lemma. *) *)
+  (* (** FIXME: Maybe don't need the GlobalInv, *)
+  (*     in which case update the specs.resources *) *)
+  (* Lemma Connection_State_relation E k r ms h : *)
+  (*     ↑KVS_InvName ⊆ E -> *)
+  (*     Global_Inv ⊢ *)
+  (*     connection_state γGsnap γT γKnownClients r (PSActive ms) -∗ *)
+  (*     ownMemUser γGauth γGsnap k h ={E}=∗ *)
+  (*     connection_state γGsnap γT γKnownClients r (PSActive ms) ∗ *)
+  (*     ownMemUser γGauth γGsnap k h ∗ *)
+  (*     ⌜k ∈ dom ms → *)
+  (*     ∀ h', ms !! k = Some h' → h' `prefix_of` h ⌝. *)
+  (* Proof. *)
+  (* Admitted.  *)
 
-  (** FIXME: Maybe don't need the GlobalInv,
-      in which case update the specs.resources *)
-    (* Lemma ConnectionState_Keys E r ms : *)
-    (*   ↑KVS_InvName ⊆ E -> *)
-    (*     GlobalInv ⊢ *)
-    (*     ConnectionState r (Active ms) ={E}=∗ *)
-    (*     ConnectionState r (Active ms) ∗ ⌜dom ms ⊆ KVS_keys⌝; *)
+  (* (** NB: not sure we will use this lemma. *) *)
+  (* (** FIXME: Maybe don't need the GlobalInv, *)
+  (*     in which case update the specs.resources *) *)
+  (* Lemma OwnMemUser_OwnLocalKey_coh k h vo c E : *)
+  (*       ↑KVS_InvName ⊆ E -> *)
+  (*       h ≠ [] -> *)
+  (*       Global_Inv ⊢ *)
+  (*       ownMemUser γGauth γGsnap k h -∗ *)
+  (*       ownCacheUser γKnownClients k c vo ={E}=∗ *)
+  (*       ownMemUser γGauth γGsnap k h ∗ *)
+  (*       ownCacheUser γKnownClients k c vo ∗ ⌜is_Some vo⌝. *)
+  (* Proof. *)
+  (* Admitted. *)
 
+  (* (** NB: not sure we will use this lemma. *) *)
+  (* (** FIXME: Maybe don't need the GlobalInv, *)
+  (*     in which case update the specs.resources *) *)
+  (*   Lemma connection_state_Keys E r ms : *)
+  (*     ↑KVS_InvName ⊆ E -> *)
+  (*       Global_Inv ⊢ *)
+  (*       connection_state γGsnap γT γKnownClients r (PSActive ms) ={E}=∗ *)
+  (*       connection_state γGsnap γT γKnownClients r (PSActive ms) ∗ *)
+  (*       ⌜dom ms ⊆ KVS_keys⌝. *)
+  (*   Proof. *)
+  (*   Admitted. *)
 
 End Global_Invariant.
